flesh out new set theory more

hol-light/polySetScript.sml
@@ -64,7 +64,6 @@ val upair_def = Define`
 val is_extensional = store_thm("is_extensional",
   ``is_set_theory ^mem ⇒ extensional mem``,
   rw[is_set_theory_def])
-val _ = export_rewrites["is_extensional"]
 
 val is_separation_sub = store_thm("is_separation_sub",
   ``is_set_theory ^mem ⇒ is_separation mem (sub mem)``,
@@ -82,41 +81,115 @@ val is_upair_upair = store_thm("is_upair_upair",
   ``is_set_theory ^mem ⇒ is_upair mem (upair mem)``,
   rw[upair_def] >> SELECT_ELIM_TAC >> fsrw_tac[SATISFY_ss][is_set_theory_def])
 
-val _ = export_rewrites["is_separation_sub","is_power_power","is_union_union","is_upair_upair"]
-
 val _ = Parse.overload_on("Sub",``sub ^mem``)
-val _ = Parse.overload_on("+",``upair ^mem``)
 val _ = Parse.overload_on("Pow",``power ^mem``)
+val _ = Parse.overload_on("+",``upair ^mem``)
+
+val mem_sub = store_thm("mem_sub",
+  ``is_set_theory ^mem ⇒ ∀x s P. mem x (Sub s P) ⇔ mem x s ∧ P x``,
+  strip_tac >> imp_res_tac is_separation_sub >> fs[is_separation_def])
+
+val mem_power = store_thm("mem_power",
+  ``is_set_theory ^mem ⇒
+    ∀x y. mem x (Pow y) ⇔ (∀b. mem b x ⇒ mem b y)``,
+  strip_tac >> imp_res_tac is_power_power >> fs[is_power_def])
+
+val mem_union = store_thm("mem_union",
+  ``is_set_theory ^mem ⇒
+    ∀x s. mem x (union mem s) ⇔ ∃a. mem x a ∧ mem a s``,
+  strip_tac >> imp_res_tac is_union_union >> fs[is_union_def])
+
+val mem_upair = store_thm("mem_upair",
+  ``is_set_theory ^mem ⇒ ∀a x y. mem a (x + y) ⇔ a = x ∨ a = y``,
+  strip_tac >> imp_res_tac is_upair_upair >> fs[is_upair_def])
 
 val empty_def = Define`
   empty ^mem = sub mem ARB (K F)`
 
 val _ = Parse.overload_on("∅",``empty ^mem``)
 
+val mem_empty = store_thm("mem_empty",
+  ``is_set_theory ^mem ⇒ ∀x. ¬mem x ∅``,
+  strip_tac >> imp_res_tac is_separation_sub >>
+  fs[empty_def,is_separation_def])
+
 val unit_def = Define`
   unit ^mem x = x + x`
 
 val _ = Parse.overload_on("Unit",``unit ^mem``)
+
+val mem_unit = store_thm("mem_unit",
+  ``is_set_theory ^mem ⇒
+    ∀x y. mem x (Unit y) ⇔ x = y``,
+  strip_tac >> imp_res_tac is_upair_upair >>
+  fs[is_upair_def,unit_def])
+
+val unit_inj = store_thm("unit_inj",
+  ``is_set_theory ^mem ⇒
+    ∀x y. Unit x = Unit y ⇔ x = y``,
+  strip_tac >>
+  imp_res_tac is_extensional >>
+  fs[extensional_def,mem_unit] >>
+  metis_tac[])
 
 val one_def = Define`
   one ^mem = Unit ∅`
 
 val _ = Parse.overload_on("One",``one ^mem``)
 
+val mem_one = store_thm("mem_one",
+  ``is_set_theory ^mem ⇒
+    ∀x. mem x One ⇔ x = ∅``,
+  strip_tac >> simp[mem_unit,one_def])
+
 val two_def = Define`
   two ^mem = ∅ + One`
 
 val _ = Parse.overload_on("Two",``two ^mem``)
+
+val mem_two = store_thm("mem_two",
+  ``is_set_theory ^mem ⇒
+    ∀x. mem x Two ⇔ x = ∅ ∨ x = One``,
+  strip_tac >> simp[mem_upair,mem_one,two_def])
 
 val pair_def = Define`
   pair ^mem x y = (Unit x) + (x + y)`
 
 val _ = Parse.overload_on(",",``pair ^mem``)
 
+val upair_inj = store_thm("upair_inj",
+  ``is_set_theory ^mem ⇒
+    ∀a b c d. a + b = c + d ⇔ a = c ∧ b = d ∨ a = d ∧ b = c``,
+  strip_tac >>
+  imp_res_tac is_extensional >>
+  fs[extensional_def,mem_upair] >>
+  metis_tac[])
+
+val unit_eq_upair = store_thm("unit_eq_upair",
+  ``is_set_theory ^mem ⇒
+    ∀x y z. Unit x = y + z ⇔ x = y ∧ y = z``,
+  strip_tac >>
+  imp_res_tac is_extensional >>
+  fs[extensional_def,mem_unit,mem_upair] >>
+  metis_tac[])
+
+val pair_inj = store_thm("pair_inj",
+  ``is_set_theory ^mem ⇒
+    ∀a b c d. (a,b) = (c,d) ⇔ a = c ∧ b = d``,
+  strip_tac >> fs[pair_def] >> rw[] >>
+  simp[upair_inj,unit_inj,unit_eq_upair] >>
+  metis_tac[])
+
 val binary_union_def = Define`
   binary_union ^mem x y = union mem (upair mem x y)`
 
 val _ = Parse.overload_on("UNION",``binary_union ^mem``)
+
+val mem_binary_union = store_thm("mem_binary_union",
+  ``is_set_theory ^mem ⇒
+    ∀a x y. mem a (x ∪ y) ⇔ mem a x ∨ mem a y``,
+  strip_tac >> fs[binary_union_def,mem_union,mem_upair] >>
+  metis_tac[])
 
 val product_def = Define`
   product ^mem x y =
@@ -124,6 +197,15 @@ val product_def = Define`
         (λa. ∃b c. mem b x ∧ mem c y ∧ a = (b,c))`
 
 val _ = Parse.overload_on("CROSS",``product ^mem``)
+
+val mem_product = store_thm("mem_product",
+  ``is_set_theory ^mem ⇒
+    ∀a x y. mem a (x × y) ⇔ ∃b c. a = (b,c) ∧ mem b x ∧ mem c y``,
+  strip_tac >> fs[product_def] >>
+  simp[mem_sub,mem_power,mem_binary_union] >>
+  rw[EQ_IMP_THM] >> TRY(metis_tac[]) >>
+  rfs[pair_def,mem_upair] >> rw[] >>
+  rfs[mem_unit,mem_upair])
 
 val relspace_def = Define`
   relspace ^mem x y = Pow (x × y)`
@@ -139,5 +221,93 @@ val _ = Parse.overload_on("Fun",``funspace ^mem``)
 
 val apply_def = Define`
   apply ^mem x y = @a. mem (y,a) x`
+
+val _ = Parse.overload_on("'",``apply ^mem``)
+
+val _ = Parse.overload_on("boolset",``Two``)
+
+val true_def = Define`
+  true ^mem = ∅`
+
+val false_def = Define`
+  false ^mem = One`
+
+val _ = Parse.overload_on("True",``true ^mem``)
+val _ = Parse.overload_on("False",``false ^mem``)
+
+val true_neq_false = store_thm("true_neq_false",
+  ``is_set_theory ^mem ⇒ True ≠ False``,
+  strip_tac >>
+  imp_res_tac mem_one >>
+  imp_res_tac mem_empty >>
+  fs[true_def,false_def,is_set_theory_def,extensional_def,one_def] >>
+  metis_tac[])
+
+val mem_boolset = store_thm("mem_boolset",
+  ``is_set_theory ^mem ⇒
+    ∀x. mem x boolset ⇔ ((x = True) ∨ (x = False))``,
+  strip_tac >> fs[mem_two,true_def,false_def])
+
+val boolean_def = Define`
+  boolean ^mem b = if b then True else False`
+
+val _ = Parse.overload_on("Boolean",``boolean ^mem``)
+
+val boolean_in_boolset = store_thm("boolean_in_boolset",
+  ``is_set_theory ^mem ⇒
+    ∀b. mem (Boolean b) boolset``,
+  strip_tac >> imp_res_tac mem_boolset >>
+  Cases >> simp[boolean_def])
+
+val boolean_eq_true = store_thm("boolean_eq_true",
+  ``is_set_theory ^mem ⇒ ∀b. Boolean b = True ⇔ b``,
+  strip_tac >> rw[boolean_def,true_neq_false])
+
+val holds_def = Define`
+  holds ^mem s x ⇔ s ' x = True`
+
+val _ = Parse.overload_on("Holds",``holds ^mem``)
+
+val abstract_def = Define`
+  abstract ^mem dom rng f = Sub (dom × rng) (λx. ∃a. x = (a,f a))`
+
+val _ = Parse.overload_on("Abstract",``abstract ^mem``)
+
+val apply_abstract = store_thm("apply_abstract",
+  ``is_set_theory ^mem ⇒
+    ∀f x s t. mem x s ∧ mem (f x) t ⇒ (Abstract s t f) ' x = f x``,
+  strip_tac >>
+  rw[apply_def,abstract_def] >>
+  SELECT_ELIM_TAC >>
+  simp[mem_sub,mem_product,pair_inj])
+
+val apply_in_rng = store_thm("apply_in_rng",
+  ``is_set_theory ^mem ⇒
+    ∀f x s t. mem x s ∧ mem f (Fun s t) ⇒
+    mem (f ' x) t``,
+  strip_tac >>
+  simp[funspace_def,mem_sub,relspace_def,
+       mem_power,apply_def,mem_product,EXISTS_UNIQUE_THM] >>
+  rw[] >> res_tac >> SELECT_ELIM_TAC >> res_tac >> rfs[pair_inj] >> metis_tac[])
+
+val abstract_in_funspace = store_thm("abstract_in_funspace",
+  ``is_set_theory ^mem ⇒
+    ∀f s t. (∀x. mem x s ⇒ mem (f x) t) ⇒ mem (Abstract s t f) (Fun s t)``,
+  strip_tac >>
+  simp[funspace_def,relspace_def,abstract_def,mem_power,mem_product,mem_sub] >>
+  simp[EXISTS_UNIQUE_THM,pair_inj])
+
+val abstract_eq = store_thm("abstract_eq",
+  ``is_set_theory ^mem ⇒
+    ∀s t1 t2 f g.
+    (∀x. mem x s ⇒ mem (f x) t1 ∧ mem (g x) t2 ∧ f x = g x)
+    ⇒ Abstract s t1 f = Abstract s t2 g``,
+  rw[] >>
+  imp_res_tac is_extensional >>
+  pop_assum mp_tac >>
+  simp[extensional_def] >>
+  disch_then kall_tac >>
+  simp[abstract_def,mem_sub,mem_product] >>
+  metis_tac[pair_inj])
 
 val _ = export_theory()
